erasure/theories/EPretty.v
@@ -84,6 +84,12 @@ Module PrintTermTree.
       let ctx' := List.map (fun d => {| decl_name := dname d; decl_body := None |}) defs in
       print_list (print_def (print_term (ctx' ++ Γ)%list true false)) (nl ^ " with ") defs.
 
+    Definition print_prim {term} (soft : term -> Tree.t) (p : @prim_val EAst.term) : Tree.t :=
+      match p.π2 return Tree.t with
+      | primIntModel f => "(int: " ^ Primitive.string_of_prim_int f ^ ")"
+      | primFloatModel f => "(float: " ^ Primitive.string_of_float f ^ ")"
+      (* | primArrayModel a => "(array:" ^ ")" *)
+      end.
 
     Fixpoint print_term (Γ : context) (top : bool) (inapp : bool) (t : term) {struct t} : Tree.t :=
     match t with
@@ -163,8 +169,7 @@ Module PrintTermTree.
     | tCoFix l n =>
       parens top ("let cofix " ^ print_defs print_term Γ l ^ nl ^
                                 " in " ^ List.nth_default (string_of_nat n) (map (string_of_name ∘ dname) l) n)
-    (* | tPrim p =>  *)
-      (* parens top (string_of_prim (print_term Γ false false) p) *)
+    | tPrim p => parens top (print_prim (print_term Γ false false) p)
     end.
   End print_term.
 
