erasure/theories/EWcbvEval.v
@@ -37,7 +37,8 @@ Definition atom `{wfl : WcbvFlags} Σ t :=
   | tBox
   | tCoFix _ _
   | tLambda _ _
-  | tFix _ _ => true
+  | tFix _ _
+  | tPrim _ => true
   | tConstruct ind c [] => negb with_constructor_as_block && isSome (lookup_constructor Σ ind c)
   | _ => false
   end.
@@ -254,7 +255,8 @@ Section Wcbv.
   (** Atoms (non redex-producing heads) applied to values are values *)
   | eval_app_cong f f' a a' :
       eval f f' ->
-      ~~ (isLambda f' || (if with_guarded_fix then isFixApp f' else isFix f') || isBox f' || isConstructApp f')  ->
+      ~~ (isLambda f' || (if with_guarded_fix then isFixApp f' else isFix f') || isBox f' || isConstructApp f'
+        || isPrimApp f')  ->
       eval a a' ->
       eval (tApp f a) (tApp f' a')
 
@@ -579,7 +581,8 @@ Section eval_rect.
                                                  else isFix f') || 
                                                  isBox f'
                                                  || 
-                                                 isConstructApp f')) 
+                                                 isConstructApp f'
+                                                 || isPrimApp f')) 
                                            (e0 : eval Σ a a'),
                                            P a a' e0
                                            → P (tApp f16 a) 
@@ -589,7 +592,7 @@ Section eval_rect.
                                     → (∀ (t : term) (i : atom Σ t),
                                          P t t (eval_atom Σ t i))
                                       → ∀ (t t0 : term) (e : eval Σ t t0),
-                                          P t t0 e.
+                                         P t t0 e.
   Proof using Type.
     intros ????????????????????? H.
     revert t t0 H.
@@ -736,8 +739,9 @@ Section Wcbv.
         + rewrite !negb_or /= in i; rtoProp; intuition auto.
         + rewrite !negb_or /= in i; rtoProp; intuition auto.
         + destruct with_guarded_fix.
-        now cbn in i. now cbn in i.
+          now cbn in i. now cbn in i.
         + constructor.
+        + cbn in i. destruct with_guarded_fix; cbn in i; rtoProp; intuition auto.
         + econstructor; auto.
       * destruct b0 as (ind & c & mdecl & idecl & cdecl & args & [H1 H2 H3 H4]).
         rewrite -[tApp _ _](mkApps_app _ (firstn n l) [a']).
@@ -1006,7 +1010,8 @@ Section Wcbv.
       rewrite !mkApps_app /=.
       eapply eval_app_cong; tea. 
       eapply IHargs => //.
-      rewrite isFixApp_mkApps // /= isConstructApp_mkApps // !negb_or. rtoProp; intuition auto.
+      rewrite isFixApp_mkApps // /= isConstructApp_mkApps // !negb_or isPrimApp_mkApps.
+      rtoProp; intuition auto.
       apply nisLambda_mkApps => //.
       destruct with_guarded_fix => //; eapply nisFix_mkApps => //.
       apply nisBox_mkApps => //.
@@ -1247,15 +1252,15 @@ Section Wcbv.
         cbn in i. rtoProp; intuition auto.
       + exfalso. rewrite !negb_or in i. specialize (IHev1 _ ev'1); noconf IHev1.
         cbn in i. rewrite guarded in i. rtoProp; intuition auto.
-        rewrite isFixApp_mkApps in H2 => //.
+        rewrite isFixApp_mkApps in H3 => //.
       + exfalso. rewrite !negb_or in i. specialize (IHev1 _ ev'1); noconf IHev1.
         cbn in i. rewrite guarded in i. rtoProp; intuition auto.
-        rewrite isFixApp_mkApps in H2 => //.
+        rewrite isFixApp_mkApps in H3 => //.
       + exfalso. rewrite !negb_or in i. specialize (IHev1 _ ev'1); noconf IHev1.
         cbn in i. rewrite unguarded in i. now cbn in i.
       + exfalso. rewrite !negb_or in i. specialize (IHev1 _ ev'1); noconf IHev1.
         cbn in i. rtoProp; intuition auto.
-        now rewrite isConstructApp_mkApps in H0.
+        now rewrite isConstructApp_mkApps in H1.
       + specialize (IHev1 _ ev'1); noconf IHev1.
         specialize (IHev2 _ ev'2); noconf IHev2.
         now assert (i0 = i) as -> by now apply uip.
